add theorem statements

TAPLFormalization/SemanticsTheorems.lean
@@ -2,3 +2,17 @@ import TAPLFormalization.Semantics
 
 theorem smallStepDeterministic : (t₁ ~> t₂) → (t₁ ~> t₃) → (t₂ = t₃) := by
   sorry
+
+def isNF (t : Term) := ∀ (t' : Term), ¬(t ~> t')
+
+inductive isValue : Term → Prop where
+  | value v : isValue (.value v)
+
+theorem isNF_iff_isValue : ∀ (t : Term), isNF t ↔ isValue t := by
+  sorry
+
+theorem NF_unique : (t ~>* u) → (t ~>* u') → isNF u → isNF u' → u = u' := by
+  sorry
+
+theorem termination : ∀ (t : Term), ∃ t', isNF t' ∧ t ~>* t' := by
+  sorry
